rocq/theories/TypeSystem/AssocCompatibilityBase.v
@@ -1,0 +1,20 @@
+From Facet.TypeSystem Require Import Lifetime Types Program TypingRules CheckerBase.
+
+Definition ty_compatible_assoc
+    (env : global_env) (Ω : outlives_ctx)
+    (T_actual T_expected : Ty) : Prop :=
+  ty_compatible Ω
+    (normalize_assoc_ty env T_actual)
+    (normalize_assoc_ty env T_expected).
+
+Definition ty_compatible_assoc_b
+    (env : global_env) (Ω : outlives_ctx)
+    (T_actual T_expected : Ty) : bool :=
+  ty_compatible_b Ω
+    (normalize_assoc_ty env T_actual)
+    (normalize_assoc_ty env T_expected).
+
+Definition ty_compatible_assoc_checked
+    (env : global_env) (Ω : outlives_ctx)
+    (T_actual T_expected : Ty) : Prop :=
+  ty_compatible_assoc_b env Ω T_actual T_expected = true.
